remove mathlib dependency

Semantics/Set.lean
@@ -1,8 +1,98 @@
--- Our only dependency on mathlib
-import Mathlib.Data.Set.Defs
+-- # Sets
+
+def Set (α : Type u) := α → Prop
+
+/-- Turn a predicate `p : α → Prop` into a set, also written as `{x | p x}` -/
+def setOf {α : Type u} (p : α → Prop) : Set α :=
+  p
+
+namespace Set
+
+/-- Membership in a set -/
+protected def Mem (s : Set α) (a : α) : Prop :=
+  s a
+
+instance : Membership α (Set α) :=
+  ⟨Set.Mem⟩
+
+theorem ext {a b : Set α} (h : ∀ (x : α), x ∈ a ↔ x ∈ b) : a = b :=
+  funext (fun x ↦ propext (h x))
+
+
+/-- The subset relation on sets. `s ⊆ t` means that all elements of `s` are elements of `t`.
+
+Note that you should **not** use this definition directly, but instead write `s ⊆ t`. -/
+protected def Subset (s₁ s₂ : Set α) :=
+  ∀ ⦃a⦄, a ∈ s₁ → a ∈ s₂
+
+/-- Porting note: we introduce `≤` before `⊆` to help the unifier when applying lattice theorems
+to subset hypotheses. -/
+instance : LE (Set α) :=
+  ⟨Set.Subset⟩
+
+instance : HasSubset (Set α) :=
+  ⟨(· ≤ ·)⟩
+
+instance : EmptyCollection (Set α) :=
+  ⟨fun _ ↦ False⟩
+
+notation "{" x " | " p "}" => setOf (λ x => p)
+
+
+/-- The universal set on a type `α` is the set containing all elements of `α`.
+
+This is conceptually the "same as" `α` (in set theory, it is actually the same), but type theory
+makes the distinction that `α` is a type while `Set.univ` is a term of type `Set α`. `Set.univ` can
+itself be coerced to a type `↥Set.univ` which is in bijection with (but distinct from) `α`. -/
+def univ : Set α := {_a | True}
+
+/-- `Set.insert a s` is the set `{a} ∪ s`.
+
+Note that you should **not** use this definition directly, but instead write `insert a s` (which is
+mediated by the `Insert` typeclass). -/
+protected def insert (a : α) (s : Set α) : Set α := {b | b = a ∨ b ∈ s}
+
+instance : Insert α (Set α) := ⟨Set.insert⟩
+
+/-- The singleton of an element `a` is the set with `a` as a single element.
+
+Note that you should **not** use this definition directly, but instead write `{a}`. -/
+protected def singleton (a : α) : Set α := {b | b = a}
+
+instance instSingletonSet : Singleton α (Set α) := ⟨Set.singleton⟩
+
+/-- The union of two sets `s` and `t` is the set of elements contained in either `s` or `t`.
+
+Note that you should **not** use this definition directly, but instead write `s ∪ t`. -/
+protected def union (s₁ s₂ : Set α) : Set α := {a | a ∈ s₁ ∨ a ∈ s₂}
+
+instance : Union (Set α) := ⟨Set.union⟩
+
+/-- The intersection of two sets `s` and `t` is the set of elements contained in both `s` and `t`.
+
+Note that you should **not** use this definition directly, but instead write `s ∩ t`. -/
+protected def inter (s₁ s₂ : Set α) : Set α := {a | a ∈ s₁ ∧ a ∈ s₂}
+
+instance : Inter (Set α) := ⟨Set.inter⟩
+
+/-- The complement of a set `s` is the set of elements not contained in `s`.
+
+Note that you should **not** use this definition directly, but instead write `sᶜ`. -/
+protected def compl (s : Set α) : Set α := {a | a ∉ s}
+
+
+/-- The difference of two sets `s` and `t` is the set of elements contained in `s` but not in `t`.
+
+Note that you should **not** use this definition directly, but instead write `s \ t`. -/
+protected def diff (s t : Set α) : Set α :=
+  λ a => a ∈ s ∧ a ∉ t
+
+instance : SDiff (Set α) := ⟨Set.diff⟩
+
+end Set
 
 /-
-  # Set theorems
+  ## Set theorems
 -/
 
 theorem Set.mem_comprehend {α : Type}
@@ -49,7 +139,7 @@ theorem Set.ite_mono (t : Set α) {s₁ s₁' s₂ s₂' : Set α}
   | Or.inr ⟨hl, hr⟩ => Or.inr ⟨h' hl, hr⟩
 
 /-
-  ### Set theoretic (partial) functions
+  ## Set theoretic (partial) functions
 
   Really these are just relations, but we can think of them as functions
 -/
