lakefile.lean
@@ -8,8 +8,6 @@ package "semantics" where
   -- ]
   -- add any additional package configuration options here
 
-require "leanprover-community" / "mathlib"
-
 @[default_target]
 lean_lib «Semantics» where
   -- add any library configuration options here
